src/Common/CommonList.v
@@ -32,6 +32,13 @@ Section Extra.
     intros. split; intro. apply in_app_or. auto. apply in_or_app. auto.
   Qed.
 
+  Corollary in_app_weak :
+    forall (x : A) l l',
+      In x l -> In x (l ++ l').
+  Proof.
+    intros. apply in_app; auto.
+  Qed.
+
   Lemma in_app_comm :
     forall (a : A) (l1 l2 : list A), In a (l1 ++ l2) <-> In a (l2 ++ l1).
   Proof.
@@ -52,34 +59,6 @@ Section Extra.
       x :: xs = [x] ++ xs.
   Proof.
     destruct xs; simpl; auto.
-  Qed.
-
-  Lemma app_length_impl :
-    forall {A B} (l1 l'1 : list A) (l2 l'2 : list B),
-      length l'1 = length l'2 ->
-      length (l'1 ++ l1) = length (l'2 ++ l2) ->
-      length l1 = length l2.
-  Proof.
-    intros * Hl Hlapp.
-    rewrite 2 app_length in Hlapp.
-    omega.
-  Qed.
-
-  Lemma length_app :
-    forall {A B} (l : list A) (l1 l2 : list B),
-      (length l = length (l1 ++ l2)) ->
-      (exists l1' l2', l = l1' ++ l2'
-                  /\ length l1' = length l1
-                  /\ length l2' = length l2).
-  Proof.
-    intros.
-    rewrite app_length in H.
-    exists (firstn (length l1) l),(skipn (length l1) l). split; [|split].
-    - symmetry. apply firstn_skipn.
-    - rewrite firstn_length. apply Min.min_l. omega.
-    - apply app_length_impl with (l'1 := firstn (length l1) l) (l'2 := l1).
-      rewrite firstn_length. apply Min.min_l. omega.
-      rewrite firstn_skipn. now rewrite app_length.
   Qed.
 
   Remark Forall_hd:
@@ -1786,6 +1765,20 @@ Section Combine.
       * apply IHl. omega.
   Qed.
 
+  Lemma in_combine_nodup :
+    forall {A B} xs ys (x : A) (y : B) y',
+      NoDup xs ->
+      In (x, y) (combine xs ys) ->
+      In (x, y') (combine xs ys) ->
+      y = y'.
+  Proof.
+    induction xs. inversion 2. intros * Hdup Hin Hin'.
+    destruct ys. inv Hin. inv Hin; inv Hin'; try congruence.
+    - inv H. inv Hdup. now take (In _ _) and apply in_combine_l in it.
+    - inv H0. inv Hdup. now take (In _ _) and apply in_combine_l in it.
+    - inv Hdup. eauto.
+  Qed.
+
 End Combine.
 
 Lemma In_combine_f_left:
@@ -1932,6 +1925,61 @@ Section SkipnDropn.
   Qed.
 
 End SkipnDropn.
+
+Section AppLength.
+  Context {A B : Type}.
+
+  Lemma app_length_impl :
+    forall (l1 l'1 : list A) (l2 l'2 : list B),
+      length l'1 = length l'2 ->
+      length (l'1 ++ l1) = length (l'2 ++ l2) ->
+      length l1 = length l2.
+  Proof.
+    intros * Hl Hlapp.
+    rewrite 2 app_length in Hlapp.
+    omega.
+  Qed.
+
+  Lemma length_app :
+    forall (l : list A) (l1 l2 : list B),
+      (length l = length (l1 ++ l2)) ->
+      (exists l1' l2', l = l1' ++ l2'
+                  /\ length l1' = length l1
+                  /\ length l2' = length l2).
+  Proof.
+    intros.
+    rewrite app_length in H.
+    exists (firstn (length l1) l),(skipn (length l1) l). split; [|split].
+    - symmetry. apply firstn_skipn.
+    - rewrite firstn_length. apply Min.min_l. omega.
+    - apply app_length_impl with (l'1 := firstn (length l1) l) (l'2 := l1).
+      rewrite firstn_length. apply Min.min_l. omega.
+      rewrite firstn_skipn. now rewrite app_length.
+  Qed.
+
+  Lemma app_length_inv1 :
+    forall (l1 l1' l2 l2' : list A),
+      l1 ++ l2 = l1' ++ l2' ->
+      length l1 = length l1' ->
+      l1 = l1'.
+  Proof.
+    intros * Happ Hlen.
+    apply f_equal with (f := firstn (length l1)) in Happ.
+    rewrite Hlen in Happ at 2.
+    do 2 rewrite firstn_app in Happ; auto.
+  Qed.
+
+  Lemma app_length_inv2:
+    forall (l1 l1' l2 l2' : list A),
+      l1 ++ l2 = l1' ++ l2' ->
+      length l1 = length l1' ->
+      l2 = l2'.
+  Proof.
+    intros * Happ Hlen.
+    apply f_equal with (f := skipn (length l1)) in Happ.
+    rewrite Hlen, skipn_app, skipn_app in Happ; auto.
+  Qed.
+End AppLength.
 
 Section Forall2.
 
@@ -3295,6 +3343,41 @@ Section OptionLists.
     setoid_rewrite Ino_In. auto using in_app_iff.
   Qed.
 
+  Lemma ino_dec:
+    forall (x : A) xos,
+      (forall x y : A, {x = y} + {x <> y}) ->
+      Ino x xos \/ ~Ino x xos.
+  Proof.
+    intros * H; rewrite Ino_In. eapply ListDec.In_decidable.
+    intros y z. destruct y as [a|], z as [b|]; try (right; congruence).
+    destruct (H a b); [left|right]; congruence.
+    now left.
+  Qed.
+
+  Lemma NoDupo_app':
+    forall (xs ws : list (option A)),
+      NoDupo xs ->
+      NoDupo ws ->
+      (forall x : A, Ino x xs -> ~ Ino x ws) ->
+      NoDupo (xs ++ ws).
+  Proof.
+    induction xs as [|[]]; intros * D1 D2 Hino; simpl; auto.
+    - constructor. inv D1. rewrite Ino_In in *. rewrite in_app.
+      intros []; auto. specialize (Hino a).
+      apply Hino; simpl; rewrite Ino_In in *; auto.
+      inv D1. apply IHxs; auto. intros. apply Hino. now right.
+    - inv D1. constructor. apply IHxs; auto. intros. apply Hino. now right.
+  Qed.
+
+  Lemma Ino_Forall:
+    forall (x : A) (xs : list (option A)) (P : option A -> Prop),
+      Forall P xs -> Ino x xs -> P (Some x).
+  Proof.
+    intros * Hforall Hin.
+    induction xs as [|a]; inversion Hin; inversion Hforall; subst; auto.
+    destruct a; simpl in *; subst; tauto.
+  Qed.
+
 End OptionLists.
 
 Ltac app_NoDupMembers_det :=
@@ -3764,24 +3847,3 @@ Section remove_member.
         right; eauto.
   Qed.
 End remove_member.
-
-(* (* Induction on a triplet of lists of the same length *) *)
-(* Section list_ind3. *)
-(*   Context {A B C : Type}. *)
-(*   Variable P : list A -> list B -> list C -> Prop. *)
-
-(*   Hypothesis Hnil : P nil nil nil. *)
-(*   Hypothesis Hcons : forall a l1 b l2 c l3, *)
-(*       P l1 l2 l3 -> P (a::l1) (b::l2) (c::l3). *)
-
-(*   Fixpoint list_ind3 l1 l2 l3 : *)
-(*     length l1 = length l2 -> *)
-(*     length l1 = length l3 -> *)
-(*     P l1 l2 l3. *)
-(*   Proof. *)
-(*     destruct l1; destruct l2; destruct l3; intros Hlen1 Hlen2; simpl in *; try congruence. *)
-(*     - apply Hcons. apply list_ind3. *)
-(*       + inv Hlen1. reflexivity. *)
-(*       + inv Hlen2. reflexivity. *)
-(*   Qed. *)
-(* End list_ind3. *)
